Proofs/Experiments/Memcpy/OmegaBench.lean
@@ -1,0 +1,55 @@
+import Arm
+import Arm.Memory.SeparateAutomation
+
+/-
+tactic execution of Lean.Parser.Tactic.omega took 6.04s
+instantiate metavars took 31.6s
+share common exprs took 5.61s
+type checking took 1.36s
+process pre-definitions took 1.02s
+-/
+set_option maxHeartbeats 0 in
+set_option trace.profiler true in
+set_option profiler true in
+theorem foo
+(s0 si : ArmState)
+(h_si_x0_nonzero : si.x0 ≠ 0)
+(h_s0_x1 : s0.x1 + 0x10#64 * (s0.x0 - si.x0) + 0x10#64 = s0.x1 + 0x10#64 * (s0.x0 - (si.x0 - 0x1#64)))
+(h_s0_x2 : s0.x2 + 0x10#64 * (s0.x0 - si.x0) + 0x10#64 = s0.x2 + 0x10#64 * (s0.x0 - (si.x0 - 0x1#64)))
+(h_assert_1 : si.x0 ≤ s0.x0)
+(h_assert_3 : si.x1 = s0.x1 + 0x10#64 * (s0.x0 - si.x0))
+(h_assert_4 : si.x2 = s0.x2 + 0x10#64 * (s0.x0 - si.x0))
+(h_assert_6 : ∀ (n : Nat) (addr : BitVec 64),
+  mem_separate' s0.x2 (0x10#64 * (s0.x0 - si.x0)).toNat addr n →
+    Memory.read_bytes n addr si.mem = Memory.read_bytes n addr s0.mem)
+(h_assert_5 : ∀ (i : BitVec 64),
+  i < s0.x0 - si.x0 →
+    Memory.read_bytes 16 (s0.x2 + 0x10#64 * i) si.mem = Memory.read_bytes 16 (s0.x1 + 0x10#64 * i) s0.mem)
+(h_pre_1 : mem_separate' s0.x1 (s0.x0.toNat * 16) s0.x2 (s0.x0.toNat * 16))
+(n : Nat)
+(addr : BitVec 64)
+(hsep : mem_separate' s0.x2 (0x10#64 * (s0.x0 - (si.x0 - 0x1#64))).toNat addr n)
+(h_le : (s0.x0 - (si.x0 - 0x1#64)).toNat ≤ s0.x0.toNat)
+(h_upper_bound : addr.toNat + n ≤ 2 ^ 64)
+(h_upper_bound₂ : s0.x2.toNat + s0.x0.toNat * 16 ≤ 2 ^ 64)
+(h_upper_bound₃ : s0.x2.toNat + (0x10#64 * (s0.x0 - (si.x0 - 0x1#64))).toNat ≤ 2 ^ 64)
+(h_width_lt : (0x10#64).toNat * (s0.x0 - (si.x0 - 0x1#64)).toNat < 2 ^ 64)
+(hmemSeparate_omega : s0.x1.toNat + s0.x0.toNat * 16 ≤ 2 ^ 64 ∧
+  s0.x2.toNat + s0.x0.toNat * 16 ≤ 2 ^ 64 ∧
+    (s0.x1.toNat + s0.x0.toNat * 16 ≤ s0.x2.toNat ∨ s0.x1.toNat ≥ s0.x2.toNat + s0.x0.toNat * 16))
+(hmemLegal_omega : s0.x1.toNat + s0.x0.toNat * 16 ≤ 2 ^ 64)
+(hmemLegal_omega : s0.x2.toNat + s0.x0.toNat * 16 ≤ 2 ^ 64)
+(hmemSeparate_omega : s0.x2.toNat + 16 % 2 ^ 64 * ((2 ^ 64 - (2 ^ 64 - 1 % 2 ^ 64 + si.x0.toNat) % 2 ^ 64 + s0.x0.toNat) % 2 ^ 64) % 2 ^ 64 ≤
+    2 ^ 64 ∧
+  addr.toNat + n ≤ 2 ^ 64 ∧
+    (s0.x2.toNat +
+          16 % 2 ^ 64 * ((2 ^ 64 - (2 ^ 64 - 1 % 2 ^ 64 + si.x0.toNat) % 2 ^ 64 + s0.x0.toNat) % 2 ^ 64) % 2 ^ 64 ≤
+        addr.toNat ∨
+      s0.x2.toNat ≥ addr.toNat + n))
+(hmemLegal_omega : s0.x2.toNat + 16 % 2 ^ 64 * ((2 ^ 64 - (2 ^ 64 - 1 % 2 ^ 64 + si.x0.toNat) % 2 ^ 64 + s0.x0.toNat) % 2 ^ 64) % 2 ^ 64 ≤
+  2 ^ 64)
+(hmemLegal_omega : addr.toNat + n ≤ 2 ^ 64) :
+ s0.x2.toNat + (0x10#64 * (s0.x0 - si.x0)).toNat ≤ 2 ^ 64 ∧
+  addr.toNat + n ≤ 2 ^ 64 ∧
+    (s0.x2.toNat + (0x10#64 * (s0.x0 - si.x0)).toNat ≤ addr.toNat ∨ s0.x2.toNat ≥ addr.toNat + n) := by
+    bv_omega
